Allow masks for NA invariants, add relational rules, update example

theories/examples/lazy.v
@@ -1,12 +1,13 @@
 From stdpp Require Import namespaces.
 From iris.base_logic Require Import invariants na_invariants.
-From self.prelude Require Import base.
 From self.prob_lang Require Import notation proofmode primitive_laws.
 From self.logrel Require Import model rel_rules rel_tactics.
 From self.examples Require Import lock.
+From self.prelude Require Import base.
+
 Set Default Proof Using "Type*".
 
-Definition lazy α : expr :=
+Definition lazy_lk α : expr :=
   let:"s" := ref NONEV in
   let: "lk" := newlock #() in
   (λ:"_u",
@@ -20,9 +21,28 @@ Definition lazy α : expr :=
     release "lk" ;;
     "r").
 
+Definition lazy α : expr :=
+  let:"s" := ref NONEV in
+  (λ:"_u",
+     match: !"s" with
+     | NONE => let: "b" := flip α in
+               "s" <- SOME "b" ;;
+               "b"
+     | SOME "b" => "b" end
+  ).
+
 Definition eager α : expr :=
   let:"b" := flip α in
   (λ:"_u", "b").
+
+Definition lazy_lk' : expr :=
+  let: "α" := alloc in lazy_lk "α".
+
+Definition lazy' : expr :=
+  let: "α" := alloc in lazy "α".
+
+Definition eager' : expr :=
+  let: "α" := alloc in eager "α".
 
 Section proofs.
   Context `{!prelogrelGS Σ}.
@@ -31,12 +51,12 @@ Section proofs.
   Definition coinN := nroot.@"coins".
 
   (* Warmup: the flips have already been resolved. *)
-  Lemma lazy_eager_refinement e1 e2 α β b bs bs' :
+  Lemma lazy_lk_eager_refinement e1 e2 α β b bs bs' :
     e1 = #lbl:α -> e2 = #lbl:β ->
     α ↪ (b::bs) ∗ β ↪ₛ (b::bs')
-    -∗ REL lazy e1 << eager e2 : lrel_unit → lrel_bool.
+    -∗ REL lazy_lk e1 << eager e2 : lrel_unit → lrel_bool.
   Proof.
-    iIntros (-> ->) "[Hα Hβ]". rewrite /lazy /eager.
+    iIntros (-> ->) "[Hα Hβ]". rewrite /lazy_lk /eager.
     rel_alloc_l l as "Hl" ; rel_pures_l ; rel_flip_r.
     rel_apply_l (refines_newlock_l coinN
                    (l ↦ NONEV ∗ α ↪ (b::bs) ∨ l ↦ SOMEV #b)%I
@@ -54,36 +74,30 @@ Section proofs.
       rel_pures_l ; rel_values.
   Qed.
 
-  Definition lazy' : expr :=
-    let: "α" := alloc in lazy "α".
-
-  Definition eager' : expr :=
-    let: "α" := alloc in eager "α".
-
-  Lemma lazy_eager_refinement' :
-    ⊢ REL lazy' << eager' : lrel_unit → lrel_bool.
+  Lemma lazy_lk_eager_refinement' :
+    ⊢ REL lazy_lk' << eager' : lrel_unit → lrel_bool.
   Proof.
-    rewrite /lazy' /eager'.
+    rewrite /lazy_lk' /eager'.
     rel_alloctape_l α as "Hα".
     rel_alloctape_r β as "Hβ".
     rel_pures_l ; rel_pures_r.
     iApply (refines_couple_tapes with "[$Hα $Hβ]"); [done|done|].
     iIntros "(%b & Hβ & Hα)".
-    iApply lazy_eager_refinement ; auto ; iFrame.
+    iApply lazy_lk_eager_refinement ; auto ; iFrame.
   Qed.
 
-  Lemma lazy_eager_refinement'' α β :
+  Lemma lazy_lk_eager_refinement'' α β :
     (REL α << β : lrel_tape)
-      ⊢ REL lazy α << eager β : lrel_unit → lrel_bool.
+      ⊢ REL lazy_lk α << eager β : lrel_unit → lrel_bool.
   Proof.
   Admitted.
 
-  Lemma eager_lazy_refinement e1 e2 α β b bs bs' :
+  Lemma eager_lazy_lk_refinement e1 e2 α β b bs bs' :
     e1 = #lbl:α -> e2 = #lbl:β ->
     α ↪ (b::bs) ∗ β ↪ₛ (b::bs')
-    -∗ REL eager e1 << lazy e2 : lrel_unit → lrel_bool.
+    -∗ REL eager e1 << lazy_lk e2 : lrel_unit → lrel_bool.
   Proof.
-    iIntros (-> ->) "[Hα Hβ]". rewrite /lazy /eager.
+    iIntros (-> ->) "[Hα Hβ]". rewrite /lazy_lk /eager.
     rel_alloc_r l as "Hl" ; rel_pures_r ; rel_flip_l.
     rel_apply_r (refines_newlock_r).
     iIntros (lk) "Hlk".
@@ -113,6 +127,51 @@ Section proofs.
     (* all: iMod ("Hclose" with "[Hlk Hl]") ; [iFrame | eauto]. *)
   (* Qed. *)
 
+  Lemma eager_lazy_lk_refinement' :
+    ⊢ REL eager' << lazy_lk' : lrel_unit → lrel_bool.
+  Proof using lockG0 prelogrelGS0 Σ.
+    rewrite /lazy_lk' /eager'.
+    rel_alloctape_l α as "Hα" ; rel_alloctape_r β as "Hβ".
+    rel_pures_l ; rel_pures_r.
+    iApply (refines_couple_tapes with "[$Hα $Hβ]"); [done|done|].
+    iIntros "(%b & Hβ & Hα)".
+    iApply eager_lazy_lk_refinement ; auto ; iFrame.
+  Qed.
+
+  Lemma eager_lazy_refinement e1 e2 α β b bs bs' :
+    e1 = #lbl:α -> e2 = #lbl:β ->
+    α ↪ (b::bs) ∗ β ↪ₛ (b::bs')
+    -∗ REL eager e1 << lazy e2 : lrel_unit → lrel_bool.
+  Proof using lockG0 prelogrelGS0 Σ.
+    iIntros (-> ->) "[Hα Hβ]". rewrite /lazy /eager.
+    rel_alloc_r l as "Hl" ; rel_pures_r ; rel_flip_l.
+    set (P := ((β ↪ₛ (b::bs') ∗ l ↦ₛ NONEV) ∨ (β ↪ₛ bs' ∗ l ↦ₛ SOMEV #b))%I).
+    (* Allocate the invariant P *)
+    iMod (na_inv_alloc prelogrelGS_nais _ coinN P with "[-]") as "#Hinv" ;
+      [by subst P ; eauto with iFrame|].
+    rel_pures_l ; rel_pures_r.
+    rel_arrow ; iIntros (v1 v2) "_". rel_pure_r.
+    (* Open the invariant. *)
+    iApply (refines_na_inv with "[$Hinv]") ; auto ; iIntros "[HP Hclose]".
+    (* Compute to strip the later off ▷ P *)
+    rel_pures_l.
+    (* Case match the different values of (! #l). *)
+    iDestruct "HP" as "[(Hβ & Hl) | (Hβ & Hl)]" ; rel_load_r ; rel_pures_r.
+    1: rel_flip_r ; rel_pures_r ; rel_store_r ; rel_pures_r.
+    (* Re-establish the invariant *)
+    all: iAssert (▷ P)%I with "[Hβ Hl]" as "HP" ; [subst P ; eauto with iFrame|].
+    (* We have two ways to finish up, either via the return rule that gives us
+       back the left-over part of the token, or via the general relational rule
+       for closing invariants. *)
+    - rel_values_na ; iIntros "Hnais".
+      iDestruct ("Hclose" with "[-]") as "Hnais" ; iFrame.
+      (* TODO: why is the iMod "Hnais" needed? Shouldn't iModIntro already
+         strip the |={⊤}=> off? *)
+      iMod "Hnais" ; iModIntro.
+      iFrame ; eauto.
+    - iApply (refines_na_close with "[$Hclose $HP]"). rel_values.
+  Qed.
+
   Lemma eager_lazy_refinement' :
     ⊢ REL eager' << lazy' : lrel_unit → lrel_bool.
   Proof.
@@ -122,6 +181,27 @@ Section proofs.
     iApply (refines_couple_tapes with "[$Hα $Hβ]"); [done|done|].
     iIntros "(%b & Hβ & Hα)".
     iApply eager_lazy_refinement ; auto ; iFrame.
+  Qed.
+
+  (* This is exactly the same as the symmetric refinement, mutatis mutandis. *)
+  Lemma lazy_eager_refinement e1 e2 α β b bs bs' :
+    e1 = #lbl:α -> e2 = #lbl:β ->
+    α ↪ (b::bs) ∗ β ↪ₛ (b::bs')
+    -∗ REL lazy e1 << eager e2 : lrel_unit → lrel_bool.
+  Proof using lockG0 prelogrelGS0 Σ.
+    iIntros (-> ->) "[Hα Hβ]". rewrite /lazy /eager.
+    rel_alloc_l l as "Hl" ; rel_pures_l ; rel_flip_r.
+    set (P := ((α ↪ (b::bs) ∗ l ↦ NONEV) ∨ (α ↪ bs ∗ l ↦ SOMEV #b))%I).
+    iMod (na_inv_alloc prelogrelGS_nais _ coinN P with "[-]") as "#Hinv" ;
+      [by subst P ; eauto with iFrame|].
+    rel_pures_l ; rel_pures_r.
+    rel_arrow ; iIntros (v1 v2) "_". rel_pure_r.
+    iApply (refines_na_inv with "[$Hinv]") ; auto ; iIntros "[HP Hclose]".
+    rel_pures_l.
+    iDestruct "HP" as "[(Hβ & Hl) | (Hβ & Hl)]" ; rel_load_l ; rel_pures_l.
+    1: rel_flip_l ; rel_pures_l ; rel_store_l ; rel_pures_l.
+    all: iAssert (▷ P)%I with "[Hβ Hl]" as "HP" ; [subst P ; eauto with iFrame|].
+    all: iApply (refines_na_close with "[$Hclose $HP]") ; rel_values.
   Qed.
 
 End proofs.
