theories/logrel/model.v
@@ -66,10 +66,10 @@ Section semtypes.
 
   Set Primitive Projections.
 
-  Definition refines_def (E : coPset) (e : expr) (e' : expr) (A : lrel Σ)
+  Definition refines_def (E F : coPset) (e : expr) (e' : expr) (A : lrel Σ)
     : iProp Σ :=
     (∀ K, refines_right K e' -∗
-          na_own prelogrelGS_nais ⊤ -∗
+          na_own prelogrelGS_nais F -∗
           WP e @ E {{ v, ∃ v', refines_right K (of_val v')
                                ∗ na_own prelogrelGS_nais ⊤
                                ∗ A v v' }})%I.
@@ -78,12 +78,12 @@ Section semtypes.
   Definition refines := unseal refines_aux.
   Definition refines_eq : refines = refines_def := seal_eq refines_aux.
 
-  Global Instance refines_ne E n :
-    Proper ((=) ==> (=) ==> (dist n) ==> (dist n)) (refines E).
+  Global Instance refines_ne E F n :
+    Proper ((=) ==> (=) ==> (dist n) ==> (dist n)) (refines E F).
   Proof. rewrite refines_eq /refines_def. solve_proper. Qed.
 
-  Global Instance refines_proper E  :
-    Proper ((=) ==> (=) ==> (≡) ==> (≡)) (refines E).
+  Global Instance refines_proper E F :
+    Proper ((=) ==> (=) ==> (≡) ==> (≡)) (refines E F).
   Proof. solve_proper_from_ne. Qed.
 
   Definition lrel_unit : lrel Σ := LRel (λ w1 w2, ⌜ w1 = #() ∧ w2 = #() ⌝%I).
@@ -91,7 +91,7 @@ Section semtypes.
   Definition lrel_int : lrel Σ := LRel (λ w1 w2, ∃ n : Z, ⌜ w1 = #n ∧ w2 = #n ⌝)%I.
 
   Definition lrel_arr (E : coPset) (A1 A2 : lrel Σ) : lrel Σ := LRel (λ w1 w2,
-    □ ∀ v1 v2, A1 v1 v2 -∗ refines E (App w1 v1) (App w2 v2) A2)%I.
+    □ ∀ v1 v2, A1 v1 v2 -∗ refines E ⊤ (App w1 v1) (App w2 v2) A2)%I.
 
   Definition lrel_ref (A : lrel Σ) : lrel Σ := LRel (λ w1 w2,
     ∃ l1 l2: loc, ⌜w1 = #l1⌝ ∧ ⌜w2 = #l2⌝ ∧
@@ -258,13 +258,23 @@ End semtypes_properties.
 (*   A at level 200, *)
 (*   format "'[hv' 'REL'  e1  '/' '<<{' id '}' '/  '  '_'  '@'  E  ':'  A ']'"). *)
 (* (￣～￣;)  OOF *)
+Notation "'REL' e1 '<<' e2 '@' E ';' F ':' A" :=
+  (refines E F e1%E e2%E (A)%lrel)
+  (at level 100, E, F at next level, e1, e2 at next level,
+   A at level 200,
+   format "'[hv' 'REL'  e1  '/' '<<'  '/  ' e2  '@'  E ';' F :  A ']'").
 Notation "'REL' e1 '<<' e2 '@' E ':' A" :=
-  (refines E e1%E e2%E (A)%lrel)
+  (refines E ⊤ e1%E e2%E (A)%lrel)
   (at level 100, E at next level, e1, e2 at next level,
    A at level 200,
    format "'[hv' 'REL'  e1  '/' '<<'  '/  ' e2  '@'  E  :  A ']'").
+Notation "'REL' e1 '<<' e2 '@' ';' F ':' A" :=
+  (refines ⊤ F e1%E e2%E (A)%lrel)
+  (at level 100, F at next level, e1, e2 at next level,
+   A at level 200,
+   format "'[hv' 'REL'  e1  '/' '<<'  '/  ' e2  '@' ';'  F  :  A ']'").
 Notation "'REL' e1 '<<' t ':' A" :=
-  (refines ⊤ e1%E t%E (A)%lrel)
+  (refines ⊤ ⊤ e1%E t%E (A)%lrel)
   (at level 100, e1, t at next level,
    A at level 200,
    format "'[hv' 'REL'  e1  '/' '<<'  '/  ' t  :  A ']'").
@@ -310,18 +320,18 @@ Section related_facts.
   (* Qed. *)
 
   (* We need this to be able to open and closed invariants in front of logrels *)
-  Lemma fupd_refines E e t A :
-    (|={E}=> refines E e t A) -∗ refines E e t A.
+  Lemma fupd_refines E F e t A :
+    (|={E}=> refines E F e t A) -∗ refines E F e t A.
   Proof.
     rewrite refines_eq /refines_def.
     iIntros "H". iIntros (j) "Hr Hna /=".
     iMod "H" as "H". iApply ("H" with "Hr Hna").
   Qed.
 
-  Global Instance elim_fupd_refines p E e t P A :
+  Global Instance elim_fupd_refines p E F e t P A :
    (* DF: look at the booleans here *)
    ElimModal True p false (|={E}=> P) P
-     (refines E e t A) (refines E e t A).
+     (refines E F e t A) (refines E F e t A).
   Proof.
     rewrite /ElimModal. intros _.
     iIntros "[HP HI]". iApply fupd_refines.
@@ -329,32 +339,62 @@ Section related_facts.
     iMod "HP"; iModIntro; by iApply "HI".
   Qed.
 
-  Global Instance elim_bupd_logrel p E e t P A :
+  Global Instance elim_bupd_logrel p E F e t P A :
    ElimModal True p false (|==> P) P
-     (refines E e t A) (refines E e t A).
+     (refines E F e t A) (refines E F e t A).
   Proof.
     rewrite /ElimModal (bupd_fupd E).
     apply: elim_fupd_refines.
   Qed.
 
   (* This + elim_modal_timless_bupd' is useful for stripping off laters of timeless propositions. *)
-  Global Instance is_except_0_logrel E e t A :
-    IsExcept0 (refines E e t A).
+  Global Instance is_except_0_logrel E F e t A :
+    IsExcept0 (refines E F e t A).
   Proof.
     rewrite /IsExcept0. iIntros "HL".
     iApply fupd_refines. by iMod "HL".
   Qed.
+
+  Lemma refines_na_inv P E F N e1 e2 A :
+    ↑N ⊆ E ->
+    ↑N ⊆ F ->
+    na_inv prelogrelGS_nais N P ∗
+    (▷ P ∗ (▷ P ∗ na_own prelogrelGS_nais (F ∖ ↑N) ={E}=∗ na_own prelogrelGS_nais F)
+     -∗ REL e1 << e2 @ E ; (F ∖ ↑N) : A)%I
+    ⊢ REL e1 << e2 @ E ; F : A.
+  Proof.
+    iIntros (NE NF) "[Hinv IH]".
+    rewrite refines_eq /refines_def.
+    iIntros (K) "Hs Hnais".
+    iMod (na_inv_acc with "Hinv Hnais") as "(HP & Hnais & Hclose)" ; auto.
+    iDestruct ("IH" with "[HP Hclose]") as "IH". 1: iFrame.
+    iApply ("IH" $! K with "Hs Hnais").
+  Qed.
+
+  Lemma refines_na_close P E F N e1 e2 A :
+    (|={E}=> REL e1 << e2 @ E ; F : A)
+    ∗ (▷ P ∗ (▷ P ∗ na_own prelogrelGS_nais (F ∖ ↑N) ={E}=∗ na_own prelogrelGS_nais F))
+    ⊢ REL e1 << e2 @ E ; (F ∖ ↑N) : A.
+  Proof.
+    iIntros "[IH [HP Hclose]]".
+    rewrite refines_eq /refines_def.
+    iIntros (K) "Hs own_FN".
+    iDestruct ("Hclose" with "[$HP $own_FN]") as "own_F".
+    iMod "own_F". iMod "IH". iApply ("IH" with "Hs own_F").
+  Qed.
+
 End related_facts.
 
 Section monadic.
   Context `{!prelogrelGS Σ}.
   Implicit Types e : expr.
 
-  Lemma refines_bind K K' E A A' e e' :
-    (REL e << e' @ E : A) -∗
+  (* PGH: could consider a version with REL v << v' @ E ; F : A *)
+  Lemma refines_bind K K' E F A A' e e' :
+    (REL e << e' @ E ; F : A) -∗
     (∀ v v', A v v' -∗
       REL fill K (of_val v) << (fill K' (of_val v')) @ E : A') -∗
-    REL fill K e << fill K' e' @ E : A'.
+    REL fill K e << fill K' e' @ E ; F : A'.
   Proof.
     iIntros "Hm Hf".
     rewrite refines_eq /refines_def /refines_right.
@@ -368,16 +408,50 @@ Section monadic.
     iApply ("Hf" with "HA Hj Hnais").
   Qed.
 
-  Lemma refines_ret E e1 e2 v1 v2 (A : lrel Σ) :
+  Lemma refines_ret_na E F e1 e2 v1 v2 (A : lrel Σ) :
     IntoVal e1 v1 →
     IntoVal e2 v2 →
-    (|={E}=> A v1 v2) -∗ REL e1 << e2 @ E : A.
+    (na_own prelogrelGS_nais F
+     ={E}=∗ na_own prelogrelGS_nais ⊤ ∗ A v1 v2) -∗
+    REL e1 << e2 @ E ; F : A.
   Proof.
     rewrite /IntoVal.
     rewrite refines_eq /refines_def.
-    iIntros (<-<-) "HA". iIntros (K) "H Hnais /=".
-    iMod "HA" as "HA".
-    iApply wp_value. iExists _. by iFrame.
+    iIntros (<-<-) "HFA". iIntros (K) "HK Hnais /=".
+    iMod ("HFA" with "Hnais") as "[HF HA]".
+    iApply wp_value. iExists _. iFrame.
+  Qed.
+
+  (* PGH: The first version of the lemma I had thought of; not sure if this is
+     actually useful. *)
+  Lemma refines_ret_na' E F e1 e2 v1 v2 (A : lrel Σ) :
+    IntoVal e1 v1 →
+    IntoVal e2 v2 →
+    (|={E}=> na_own prelogrelGS_nais (⊤ ∖ F) ∗ A v1 v2) -∗
+    REL e1 << e2 @ E ; F : A.
+  Proof.
+    rewrite /IntoVal.
+    rewrite refines_eq /refines_def.
+    iIntros (<-<-) "HFA". iIntros (j) "Hj Hnais /=".
+    iMod "HFA" as "[HF HA]".
+    iApply wp_value. iExists _. iFrame.
+    assert (F ## (⊤ ∖ F)) as H by set_solver.
+    iPoseProof (na_own_union _ _ _ H with "[$HF $Hnais]") as "HL".
+    assert ((F ∪ (⊤ ∖ F)) = ⊤) as ->. 2: done.
+    rewrite union_comm_L.
+    rewrite difference_union_L.
+    set_solver.
+  Qed.
+
+  Lemma refines_ret E e1 e2 v1 v2 (A : lrel Σ) :
+    IntoVal e1 v1 →
+    IntoVal e2 v2 →
+    (|={E}=> A v1 v2) -∗
+    REL e1 << e2 @ E : A.
+  Proof.
+    iIntros (hv1 hv2) "HA".
+    iApply refines_ret_na.
+    iIntros "Hnais". iMod "HA". now iFrame.
   Qed.
 
 End monadic.
