theories/logrel/rel_rules.v
@@ -21,24 +21,23 @@ Section rules.
 
   (** ** Forward reductions on the LHS *)
 
-  Lemma refines_pure_l E n
+  Lemma refines_pure_l E F n
     (K' : list ectx_item) e e' t A ϕ :
     PureExec ϕ n e e' →
     ϕ →
-    ▷^n (REL fill K' e' << t @ E : A)
-    ⊢ REL fill K' e << t @ E : A.
+    ▷^n (REL fill K' e' << t @ E ; F : A)
+    ⊢ REL fill K' e << t @ E ; F : A.
   Proof.
     intros Hpure Hϕ.
     rewrite refines_eq /refines_def.
     iIntros "IH" (j) "Hs Hnais".
-    wp_pures.
-    iApply ("IH" with "Hs Hnais").
+    wp_pures. iApply ("IH" with "Hs Hnais").
   Qed.
 
-  Lemma refines_wp_l E K e1 t A :
+  Lemma refines_wp_l E F K e1 t A :
     (WP e1 @ E {{ v,
-        REL fill K (of_val v) << t @ E : A }})%I -∗
-    REL fill K e1 << t @ E : A.
+        REL fill K (of_val v) << t @ E ; F : A }})%I -∗
+    REL fill K e1 << t @ E ; F : A.
   Proof.
     rewrite refines_eq /refines_def.
     iIntros "He" (K') "Hs Hnais /=".
@@ -48,13 +47,13 @@ Section rules.
     iApply ("Hv" with "Hs Hnais").
   Qed.
 
-  Lemma refines_atomic_l (E1 E2 : coPset) K e1 t A
+  Lemma refines_atomic_l (E1 E2 F : coPset) K e1 t A
     (Hatomic : Atomic WeaklyAtomic e1) :
     (∀ K', refines_right K' t ={E1,E2}=∗
              WP e1 @ E2 {{ v,
               |={E2, E1}=> ∃ t', refines_right K' t' ∗
-              REL fill K (of_val v) << t' @ E1 : A }})%I -∗
-   REL fill K e1 << t @ E1 : A.
+              REL fill K (of_val v) << t' @ E1 ; F : A }})%I -∗
+   REL fill K e1 << t @ E1 ; F: A.
   Proof.
     rewrite refines_eq /refines_def.
     iIntros "Hlog" (K') "Hs Hnais /=".
@@ -68,12 +67,12 @@ Section rules.
 
   (** ** Forward reductions on the RHS *)
 
-  Lemma refines_pure_r E K' e e' t A n
+  Lemma refines_pure_r E F K' e e' t A n
     (Hspec : nclose specN ⊆ E) ϕ :
     PureExec ϕ n e e' →
     ϕ →
-    (REL t << fill K' e' @ E : A)
-    ⊢ REL t << fill K' e @ E : A.
+    (REL t << fill K' e' @ E ; F : A)
+    ⊢ REL t << fill K' e @ E ; F : A.
   Proof.
     rewrite refines_eq /refines_def => Hpure Hϕ.
     iIntros "Hlog" (j) "Hj Hnais /=".
@@ -88,10 +87,10 @@ Section rules.
   Definition refines_right_bind' := refines_right_bind.
 
   (* A helper lemma for proving the stateful reductions for the RHS below *)
-  Lemma refines_step_r E K' e1 e2 A :
+  Lemma refines_step_r E F K' e1 e2 A :
     (∀ k, refines_right k e2 ={E}=∗
-         ∃ v, refines_right k (of_val v) ∗ REL e1 << fill K' (of_val v) @ E : A) -∗
-    REL e1 << fill K' e2 @ E : A.
+         ∃ v, refines_right k (of_val v) ∗ REL e1 << fill K' (of_val v) @ E ; F : A) -∗
+    REL e1 << fill K' e2 @ E ; F : A.
   Proof.
     rewrite refines_eq /refines_def /=.
     iIntros "He" (K'') "Hs Hnais /=".
@@ -102,11 +101,11 @@ Section rules.
     by iApply "He".
   Qed.
 
-  Lemma refines_alloc_r E K e v t A
+  Lemma refines_alloc_r E F K e v t A
     (Hmasked : nclose specN ⊆ E) :
     IntoVal e v →
-    (∀ l : loc, l ↦ₛ v -∗ REL t << fill K (of_val #l) @ E : A)%I
-    -∗ REL t << fill K (ref e) @ E : A.
+    (∀ l : loc, l ↦ₛ v -∗ REL t << fill K (of_val #l) @ E ; F : A)%I
+    -∗ REL t << fill K (ref e) @ E ; F : A.
   Proof.
     rewrite /IntoVal. intros <-.
     iIntros "Hlog". simpl.
@@ -116,11 +115,11 @@ Section rules.
     iModIntro. iExists _. iFrame. by iApply "Hlog".
   Qed.
 
-  Lemma refines_load_r E K l q v t A
+  Lemma refines_load_r E F K l q v t A
     (Hmasked : nclose specN ⊆ E) :
     l ↦ₛ{q} v -∗
-    (l ↦ₛ{q} v -∗ REL t << fill K (of_val v) @ E : A)
-    -∗ REL t << (fill K !#l) @ E : A.
+    (l ↦ₛ{q} v -∗ REL t << fill K (of_val v) @ E ; F : A)
+    -∗ REL t << (fill K !#l) @ E ; F : A.
   Proof.
     iIntros "Hl Hlog".
     iApply refines_step_r.
@@ -129,12 +128,12 @@ Section rules.
     iModIntro. iExists _. iFrame. by iApply "Hlog".
   Qed.
 
-  Lemma refines_store_r E K l e e' v v' A
+  Lemma refines_store_r E F K l e e' v v' A
     (Hmasked : nclose specN ⊆ E) :
     IntoVal e' v' →
     l ↦ₛ v -∗
-    (l ↦ₛ v' -∗ REL e << fill K (of_val #()) @ E : A) -∗
-    REL e << fill K (#l <- e') @ E : A.
+    (l ↦ₛ v' -∗ REL e << fill K (of_val #()) @ E ; F : A) -∗
+    REL e << fill K (#l <- e') @ E ; F : A.
   Proof.
     rewrite /IntoVal. iIntros (<-) "Hl Hlog".
     iApply refines_step_r.
@@ -143,10 +142,10 @@ Section rules.
     by iApply "Hlog".
   Qed.
 
-  Lemma refines_alloctape_r E K t A
+  Lemma refines_alloctape_r E F K t A
     (Hmasked : nclose specN ⊆ E) :
-    (∀ α : loc, α ↪ₛ [] -∗ REL t << fill K (of_val #lbl:α) @ E : A)%I
-    -∗ REL t << fill K alloc @ E : A.
+    (∀ α : loc, α ↪ₛ [] -∗ REL t << fill K (of_val #lbl:α) @ E ; F : A)%I
+    -∗ REL t << fill K alloc @ E ; F : A.
   Proof.
     rewrite /IntoVal.
     iIntros "Hlog".
@@ -156,11 +155,11 @@ Section rules.
     iModIntro. iExists _. iFrame. by iApply "Hlog".
   Qed.
 
-  Lemma refines_flip_r E K α b bs t A
+  Lemma refines_flip_r E F K α b bs t A
     (Hmasked : nclose specN ⊆ E) :
     α ↪ₛ (b :: bs)
-    -∗ (α ↪ₛ bs -∗ REL t << fill K (of_val #b) @ E : A)
-    -∗ REL t << (fill K (flip #lbl:α)) @ E : A.
+    -∗ (α ↪ₛ bs -∗ REL t << fill K (of_val #b) @ E ; F : A)
+    -∗ REL t << (fill K (flip #lbl:α)) @ E ; F : A.
   Proof.
     iIntros "Hα Hlog".
     iApply refines_step_r.
@@ -186,63 +185,63 @@ Section rules.
 
   (** ** Stateful reductions on the LHS *)
 
-  Lemma refines_alloc_l K E e v t A :
+  Lemma refines_alloc_l K E F e v t A :
     IntoVal e v →
     (▷ (∀ l : loc, l ↦ v -∗
-           REL fill K (of_val #l) << t @ E : A))
-    -∗ REL fill K (ref e) << t @ E : A.
+           REL fill K (of_val #l) << t @ E ; F : A))
+    -∗ REL fill K (ref e) << t @ E ; F : A.
   Proof.
     iIntros (<-) "Hlog".
     iApply refines_wp_l.
     wp_alloc l. by iApply "Hlog".
   Qed.
 
-  Lemma refines_load_l K E l q t A :
+  Lemma refines_load_l K E F l q t A :
     (∃ v',
       ▷(l ↦{q} v') ∗
-      ▷(l ↦{q} v' -∗ (REL fill K (of_val v') << t @ E : A)))
-    -∗ REL fill K (! #l) << t @ E : A.
+      ▷(l ↦{q} v' -∗ (REL fill K (of_val v') << t @ E ; F : A)))
+    -∗ REL fill K (! #l) << t @ E ; F : A.
   Proof.
     iIntros "[%v' [Hl Hlog]]".
     iApply refines_wp_l.
     wp_load. by iApply "Hlog".
   Qed.
 
-  Lemma refines_store_l K E l e v' t A :
+  Lemma refines_store_l K E F l e v' t A :
     IntoVal e v' →
     (∃ v, ▷ l ↦ v ∗
-      ▷(l ↦ v' -∗ REL fill K (of_val #()) << t @ E : A))
-    -∗ REL fill K (#l <- e) << t @ E : A.
+      ▷(l ↦ v' -∗ REL fill K (of_val #()) << t @ E ; F : A))
+    -∗ REL fill K (#l <- e) << t @ E ; F : A.
   Proof.
     iIntros (<-) "[%v [Hl Hlog]]".
     iApply refines_wp_l.
     wp_store. by iApply "Hlog".
   Qed.
 
-  Lemma refines_alloctape_l K E t A :
+  Lemma refines_alloctape_l K E F t A :
     (▷ (∀ α : loc, α ↪ [] -∗
-           REL fill K (of_val #lbl:α) << t @ E : A))
-    -∗ REL fill K alloc << t @ E : A.
+           REL fill K (of_val #lbl:α) << t @ E ; F : A))%I
+    -∗ REL fill K alloc << t @ E ; F : A.
   Proof.
     iIntros "Hlog".
     iApply refines_wp_l.
     by wp_apply (wp_alloc_tape with "[//]").
   Qed.
 
-  Lemma refines_flip_l E K α t A b bs :
+  Lemma refines_flip_l E F K α b bs t A :
     (▷ α ↪ (b :: bs) ∗
-       ▷ (α ↪ bs -∗ REL fill K (of_val #b) << t @ E : A))
-    -∗ REL fill K (flip #lbl:α) << t @ E : A.
+     ▷ (α ↪ bs -∗ REL fill K (of_val #b) << t @ E ; F : A))
+    -∗ REL fill K (flip #lbl:α) << t @ E ; F : A.
   Proof.
     iIntros "[Hα Hlog]".
     iApply refines_wp_l.
     by wp_apply (wp_flip with "Hα").
   Qed.
 
-  Lemma refines_wand E e1 e2 A A' :
-    (REL e1 << e2 @ E : A) -∗
+  Lemma refines_wand E F e1 e2 A A' :
+    (REL e1 << e2 @ E ; F : A) -∗
     (∀ v1 v2, A v1 v2 ={E}=∗ A' v1 v2) -∗
-    REL e1 << e2 @ E : A'.
+    REL e1 << e2 @ E ; F : A'.
   Proof.
     iIntros "He HAA".
     iApply (refines_bind [] [] with "He").
@@ -262,13 +261,13 @@ Section rules.
     by iApply refines_ret.
   Qed.
 
-  Lemma refines_couple_tapes E e1 e2 A α αₛ bs bsₛ
+  Lemma refines_couple_tapes E F e1 e2 A α αₛ bs bsₛ
     (Hmasked : nclose specN ⊆ E) :
     to_val e1 = None →
     ((αₛ ↪ₛ bsₛ ∗ α ↪ bs ∗
        ((∃ b, αₛ ↪ₛ (bsₛ ++ [b]) ∗ α ↪ (bs ++ [b]))
-       -∗ REL e1 << e2 @ E : A)))
-    ⊢ REL e1 << e2 @ E : A.
+       -∗ REL e1 << e2 @ E ; F : A)))
+    ⊢ REL e1 << e2 @ E ; F : A.
   Proof.
     iIntros (e1ev) "(Hαs & Hα & Hlog)".
     (* TODO: a separate [refines] lemma in [model] *)
